4.3 invariant hoisting (WIP)

examples/rel/Benton2004.RHL.Examples.fst
@@ -77,3 +77,130 @@ let sec42_ex5
 = sec42_ex1 x y z;
   sec42_ex4 x y
   // r_seq automatically applied
+
+let sec43_phi
+  (i n x y: var)
+: GTot (gexp bool)
+= gand
+    (geq (gvar i Left) (gvar i Right))
+    (gand
+      (geq (gvar n Left) (gvar n Right))
+      (geq (gvar y Left) (gvar y Right))
+    )
+
+let sec43_left
+  (i n x y: var)
+: Tot computation
+= while (eop op_LessThan (evar i) (evar n)) (seq
+    (assign x (eop op_Addition (evar y) (const 1)))
+    (assign i (eop op_Addition (evar i) (evar x)))
+  )
+
+let sec43_right
+  (i n x y: var)
+: Tot computation
+= seq
+  (assign x (eop op_Addition (evar y) (const 1)))
+  (while (eop op_LessThan (evar i) (evar n))
+    (assign i (eop op_Addition (evar i) (evar x)))
+  )
+
+(* Proof becomes really intractable. Thus let's design a better rule for assignment. *)
+
+let r_ass
+  (x y: var)
+  (e e' : exp int)
+  (p p': gexp bool)
+: Lemma
+  (requires (
+    included
+      p
+      (gsubst (gsubst p' x Left (exp_to_gexp e Left)) y Right (exp_to_gexp e' Right))
+  ))
+  (ensures (exec_equiv
+    p
+    p'
+    (assign x e)
+    (assign y e')
+  ))
+= Benton2004.RHL.r_ass x y e e' p'
+
+let r_dassl
+  (x: var)
+  (e: exp int)
+  (phi phi': gexp bool)
+: Lemma
+  (requires (
+    included phi (gsubst phi' x Left (exp_to_gexp e Left))
+  ))
+  (ensures (exec_equiv phi phi' (assign x e) skip))
+= Benton2004.RHL.r_dassl x e phi'
+
+let flip_flip
+  (phi: gexp bool)
+: Lemma
+  (flip (flip phi) == phi)
+  [SMTPat (flip (flip phi))]
+= gfeq2 (flip (flip phi)) phi
+
+let r_dassr
+  (x: var)
+  (e: exp int)
+  (phi phi' : gexp bool)
+: Lemma
+  (requires (
+    included phi (gsubst phi' x Right (exp_to_gexp e Right))
+  ))
+  (ensures (exec_equiv phi phi' skip (assign x e)))
+= r_dassl x e (flip phi) (flip phi')
+
+#set-options "--z3rlimit 64"
+
+let sec43
+  (i n x y: var)
+  (diffs: squash (List.Tot.noRepeats [i; n; x; y] == true))
+: Lemma
+  (ensures (
+    exec_equiv
+      (sec43_phi i n x y)
+      (sec43_phi i n x y)
+      (sec43_left i n x y)
+      (sec43_right i n x y)
+  ))
+= let phi = sec43_phi i n x y in
+  let l = sec43_left i n x y in
+  let r = sec43_right i n x y in
+  let phi_per : squash (is_per phi) = () in
+  let phi_interp : squash (interpolable phi) = () in
+  let cond = eop op_LessThan (evar i) (evar n) in
+  let lbody_phi = gand phi (gand (exp_to_gexp cond Left) (exp_to_gexp cond Right)) in
+  let lbody_phi' = gand phi (geq (exp_to_gexp cond Left) (exp_to_gexp cond Right)) in
+  let asx_e = eop op_Addition (evar y) (const 1) in
+  let asx = assign x asx_e in
+  let lbody_phi12 = gand lbody_phi' (geq (gvar x Left) (gvar x Right)) in
+  let asi_e = eop op_Addition (evar i) (evar x) in
+  let asi = assign i asi_e in
+  let lbody = seq asx asi in
+  let rloop = while cond asi in
+  let _ : squash (exec_equiv phi phi l (seq skip l)) =
+    r_ass x x asx_e asx_e lbody_phi lbody_phi12;
+    r_ass i i asi_e asi_e lbody_phi12 lbody_phi';
+    r_while cond cond lbody lbody phi;
+    d_su1 l phi phi;
+    phi_per;
+    phi_interp;
+    assert (exec_equiv phi phi l (seq skip l))
+  in
+  let _ : squash (exec_equiv phi phi (seq skip l) r) =
+    let gi () : Lemma (x <> i /\ x <> n /\ x <> y) =
+      diffs;
+      ()
+    in
+    gi ();
+    r_dassr x asx_e phi phi;
+    assume (exec_equiv phi phi l rloop);
+    r_seq phi phi phi skip asx l rloop
+  in
+  phi_per;
+  phi_interp;
+  ()
